syntax.v
@@ -1,63 +1,62 @@
-Require Export unscoped.
-Require Export header_extensible.
+Require Export unscoped header_extensible.
+
+(*Require Export univ implicative.*)
 
 Class Signature := B_S { Funcs : Type; fun_ar : Funcs -> nat ; Preds : Type; pred_ar : Preds -> nat }.
 Context {Sigma : Signature}.
-Definition V n t := Vector.t t n.
-Definition V_map {term : Type} (f : term -> term ) {n:nat} (v : Vector.t term n) := Vector.map f v.
 
 Section term.
 Inductive term  : Type :=
   | var_term : ( fin ) -> term 
-  | Func : forall (f : Funcs), ( term   ) -> term .
+  | Func : forall (f : Funcs), ( vect (fun_ar f) (term  ) ) -> term .
 
-Lemma congr_Func { f : Funcs }  { s0 : term   } { t0 : term   } (H1 : s0 = t0) : Func  f s0 = Func  f t0 .
+Lemma congr_Func { f : Funcs }  { s0 : vect (fun_ar f) (term  ) } { t0 : vect (fun_ar f) (term  ) } (H1 : s0 = t0) : Func  f s0 = Func  f t0 .
 Proof. congruence. Qed.
 
 Fixpoint subst_term   (sigmaterm : ( fin ) -> term ) (s : term ) : term  :=
     match s return term  with
     | var_term  s => sigmaterm s
-    | Func  f s0 => Func  f ((subst_term sigmaterm) s0)
+    | Func  f s0 => Func  f ((vect_map (subst_term sigmaterm)) s0)
     end.
 
-(* Definition up_term_term   (sigma : ( fin ) -> term ) : ( fin ) -> term  :=
-  (scons) ((var_term ) (var_zero)) ((funcomp) (subst_term ((funcomp) (var_term (_)) (shift))) sigma).
+Definition up_term_term   (sigma : ( fin ) -> term ) : ( fin ) -> term  :=
+  (scons) ((var_term ) (var_zero)) ((funcomp) (subst_term ((funcomp) (var_term ) (shift))) sigma).
 
 Definition upId_term_term  (sigma : ( fin ) -> term ) (Eq : forall x, sigma x = (var_term ) x) : forall x, (up_term_term sigma) x = (var_term ) x :=
   fun n => match n with
-  | S fin_n => (ap) (subst_term ((funcomp) (var_term (_)) (shift))) (Eq fin_n)
-  | 0 => eq_refl
+  | S fin_n => (ap) (subst_term ((funcomp) (var_term ) (shift))) (Eq fin_n)
+  | 0  => eq_refl
   end.
 
-Fixpoint idSubst_term  (sigmaterm : ( fin ) -> term ) (Eqterm : forall x, sigmaterm x = (var_term ) x) (s : term ) : subst_term sigmaterm s = s :=
+(* Fixpoint idSubst_term  (sigmaterm : ( fin ) -> term ) (Eqterm : forall x, sigmaterm x = (var_term ) x) (s : term ) : subst_term sigmaterm s = s :=
     match s return subst_term sigmaterm s = s with
     | var_term  s => Eqterm s
-    | Func  f s0 => congr_Func ((idSubst_term sigmaterm Eqterm) s0)
-    end.
+    | Func  f s0 => congr_Func ((vect_id (idSubst_term sigmaterm Eqterm)) s0)
+    end. *)
 
 Definition upExt_term_term   (sigma : ( fin ) -> term ) (tau : ( fin ) -> term ) (Eq : forall x, sigma x = tau x) : forall x, (up_term_term sigma) x = (up_term_term tau) x :=
   fun n => match n with
-  | S fin_n => (ap) (subst_term ((funcomp) (var_term (_)) (shift))) (Eq fin_n)
-  | 0 => eq_refl
+  | S fin_n => (ap) (subst_term ((funcomp) (var_term ) (shift))) (Eq fin_n)
+  | 0  => eq_refl
   end.
 
-Fixpoint ext_term   (sigmaterm : ( fin ) -> term ) (tauterm : ( fin ) -> term ) (Eqterm : forall x, sigmaterm x = tauterm x) (s : term ) : subst_term sigmaterm s = subst_term tauterm s :=
+(* Fixpoint ext_term   (sigmaterm : ( fin ) -> term ) (tauterm : ( fin ) -> term ) (Eqterm : forall x, sigmaterm x = tauterm x) (s : term ) : subst_term sigmaterm s = subst_term tauterm s :=
     match s return subst_term sigmaterm s = subst_term tauterm s with
     | var_term  s => Eqterm s
-    | Func  f s0 => congr_Func ((ext_term sigmaterm tauterm Eqterm) s0)
+    | Func  f s0 => congr_Func ((vect_ext (ext_term sigmaterm tauterm Eqterm)) s0)
     end.
 
 Fixpoint compSubstSubst_term    (sigmaterm : ( fin ) -> term ) (tauterm : ( fin ) -> term ) (thetaterm : ( fin ) -> term ) (Eqterm : forall x, ((funcomp) (subst_term tauterm) sigmaterm) x = thetaterm x) (s : term ) : subst_term tauterm (subst_term sigmaterm s) = subst_term thetaterm s :=
     match s return subst_term tauterm (subst_term sigmaterm s) = subst_term thetaterm s with
     | var_term  s => Eqterm s
-    | Func  f s0 => congr_Func ((compSubstSubst_term sigmaterm tauterm thetaterm Eqterm) s0)
+    | Func  f s0 => congr_Func ((vect_comp (compSubstSubst_term sigmaterm tauterm thetaterm Eqterm)) s0)
     end.
 
 Definition up_subst_subst_term_term    (sigma : ( fin ) -> term ) (tauterm : ( fin ) -> term ) (theta : ( fin ) -> term ) (Eq : forall x, ((funcomp) (subst_term tauterm) sigma) x = theta x) : forall x, ((funcomp) (subst_term (up_term_term tauterm)) (up_term_term sigma)) x = (up_term_term theta) x :=
   fun n => match n with
-  | S fin_n => (eq_trans) (compSubstSubst_term ((funcomp) (var_term (_)) (shift)) (up_term_term tauterm) ((funcomp) (up_term_term tauterm) (shift)) (fun x => eq_refl) (sigma fin_n)) ((eq_trans) ((eq_sym) (compSubstSubst_term tauterm ((funcomp) (var_term (_)) (shift)) ((funcomp) (subst_term ((funcomp) (var_term (_)) (shift))) tauterm) (fun x => eq_refl) (sigma fin_n))) ((ap) (subst_term ((funcomp) (var_term (_)) (shift))) (Eq fin_n)))
-  | 0 => eq_refl
-  end.
+  | S fin_n => (eq_trans) (compSubstSubst_term ((funcomp) (var_term ) (shift)) (up_term_term tauterm) ((funcomp) (up_term_term tauterm) (shift)) (fun x => eq_refl) (sigma fin_n)) ((eq_trans) ((eq_sym) (compSubstSubst_term tauterm ((funcomp) (var_term ) (shift)) ((funcomp) (subst_term ((funcomp) (var_term ) (shift))) tauterm) (fun x => eq_refl) (sigma fin_n))) ((ap) (subst_term ((funcomp) (var_term ) (shift))) (Eq fin_n)))
+  | 0  => eq_refl
+  end. 
 
 Lemma instId_term  : subst_term (var_term ) = id .
 Proof. exact ((FunctionalExtensionality.functional_extensionality _ _ ) (fun x => idSubst_term (var_term ) (fun n => eq_refl) ((id) x))). Qed.
@@ -70,12 +69,12 @@ Proof. exact (compSubstSubst_term sigmaterm tauterm (_) (fun n => eq_refl) s). Q
 
 Lemma compComp'_term    (sigmaterm : ( fin ) -> term ) (tauterm : ( fin ) -> term ) : (funcomp) (subst_term tauterm) (subst_term sigmaterm) = subst_term ((funcomp) (subst_term tauterm) sigmaterm) .
 Proof. exact ((FunctionalExtensionality.functional_extensionality _ _ ) (fun n => compComp_term sigmaterm tauterm n)). Qed.
- *)
+*)
 End term.
 
 Section form_univ.
 Variable form : Type.
-(*
+
 Variable subst_form : forall   (sigmaterm : ( fin ) -> term ) (s : form ), form .
 
 Variable idSubst_form : forall  (sigmaterm : ( fin ) -> term ) (Eqterm : forall x, sigmaterm x = (var_term ) x) (s : form ), subst_form sigmaterm s = s.
@@ -83,11 +82,11 @@ Variable idSubst_form : forall  (sigmaterm : ( fin ) -> term ) (Eqterm : forall 
 Variable ext_form : forall   (sigmaterm : ( fin ) -> term ) (tauterm : ( fin ) -> term ) (Eqterm : forall x, sigmaterm x = tauterm x) (s : form ), subst_form sigmaterm s = subst_form tauterm s.
 
 Variable compSubstSubst_form : forall    (sigmaterm : ( fin ) -> term ) (tauterm : ( fin ) -> term ) (thetaterm : ( fin ) -> term ) (Eqterm : forall x, ((funcomp) (subst_term tauterm) sigmaterm) x = thetaterm x) (s : form ), subst_form tauterm (subst_form sigmaterm s) = subst_form thetaterm s.
-*)
-Inductive form_univ  : Type :=
-  | All : ( form ) -> form_univ .
 
-(* Variable retract_form_univ : retract form_univ form.
+Inductive form_univ  : Type :=
+  | All : ( form   ) -> form_univ .
+
+Variable retract_form_univ : retract form_univ form.
 
 Definition All_  (s0 : form  ) : _ :=
   inj (All s0).
@@ -95,7 +94,7 @@ Definition All_  (s0 : form  ) : _ :=
 Lemma congr_All_  { s0 : form   } { t0 : form   } (H1 : s0 = t0) : All_  s0 = All_  t0 .
 Proof. congruence. Qed.
 
-Variable retract_ren_form : forall   (xiterm : ( fin ) -> fin) s, ren_form xiterm (inj s) = ren_form_univ xiterm s.
+(* Variable retract_ren_form : forall   (xiterm : ( fin ) -> fin) s, ren_form xiterm (inj s) = ren_form_univ xiterm s. *)
 
 Definition subst_form_univ   (sigmaterm : ( fin ) -> term ) (s : form_univ ) : form  :=
     match s return form  with
@@ -114,7 +113,7 @@ Definition ext_form_univ   (sigmaterm : ( fin ) -> term ) (tauterm : ( fin ) -> 
     | All  s0 => congr_All_ ((ext_form (up_term_term sigmaterm) (up_term_term tauterm) (upExt_term_term (_) (_) Eqterm)) s0)
     end.
 
-Definition compSubstSubst_form_univ    (sigmaterm : ( fin ) -> term ) (tauterm : ( fin ) -> term ) (thetaterm : ( fin ) -> term ) (Eqterm : forall x, ((funcomp) (subst_term tauterm) sigmaterm) x = thetaterm x) (s : form_univ ) : subst_form tauterm (subst_form_univ sigmaterm s) = subst_form_univ thetaterm s :=
+(* Definition compSubstSubst_form_univ    (sigmaterm : ( fin ) -> term ) (tauterm : ( fin ) -> term ) (thetaterm : ( fin ) -> term ) (Eqterm : forall x, ((funcomp) (subst_term tauterm) sigmaterm) x = thetaterm x) (s : form_univ ) : subst_form tauterm (subst_form_univ sigmaterm s) = subst_form_univ thetaterm s :=
     match s return subst_form tauterm (subst_form_univ sigmaterm s) = subst_form_univ thetaterm s with
     | All  s0 => (eq_trans) (retract_subst_form (_) (All (_))) (congr_All_ ((compSubstSubst_form (up_term_term sigmaterm) (up_term_term tauterm) (up_term_term thetaterm) (up_subst_subst_term_term (_) (_) (_) Eqterm)) s0))
     end.
@@ -130,27 +129,27 @@ Proof. exact ((FunctionalExtensionality.functional_extensionality _ _ ) (fun n =
 
 Definition isIn_form_form_univ (s : form) (t : form_univ) : Prop :=
   match t with
-  | All t0 => s = t0
-  end. *)
-
+  | All t0  => s = t0
+  end.
+*)
 End form_univ.
 
-Section form_imp.
+Section form_implicative.
 Variable form : Type.
-(*
+
 Variable subst_form : forall   (sigmaterm : ( fin ) -> term ) (s : form ), form .
 
 Variable idSubst_form : forall  (sigmaterm : ( fin ) -> term ) (Eqterm : forall x, sigmaterm x = (var_term ) x) (s : form ), subst_form sigmaterm s = s.
 
 Variable ext_form : forall   (sigmaterm : ( fin ) -> term ) (tauterm : ( fin ) -> term ) (Eqterm : forall x, sigmaterm x = tauterm x) (s : form ), subst_form sigmaterm s = subst_form tauterm s.
 
-Variable compSubstSubst_form : forall    (sigmaterm : ( fin ) -> term ) (tauterm : ( fin ) -> term ) (thetaterm : ( fin ) -> term ) (Eqterm : forall x, ((funcomp) (subst_term tauterm) sigmaterm) x = thetaterm x) (s : form ), subst_form tauterm (subst_form sigmaterm s) = subst_form thetaterm s.
-*)
-Inductive form_imp  : Type :=
-  | Fal : form_imp 
-  | Impl : ( form   ) -> ( form   ) -> form_imp .
-(* 
-Variable retract_form_imp : retract form_imp form.
+(* Variable compSubstSubst_form : forall    (sigmaterm : ( fin ) -> term ) (tauterm : ( fin ) -> term ) (thetaterm : ( fin ) -> term ) (Eqterm : forall x, ((funcomp) (subst_term tauterm) sigmaterm) x = thetaterm x) (s : form ), subst_form tauterm (subst_form sigmaterm s) = subst_form thetaterm s. *)
+
+Inductive form_implicative  : Type :=
+  | Fal : form_implicative 
+  | Impl : ( form   ) -> ( form   ) -> form_implicative .
+
+Variable retract_form_implicative : retract form_implicative form.
 
 Definition Fal_  : _ :=
   inj (Fal ).
@@ -164,108 +163,108 @@ Proof. congruence. Qed.
 Lemma congr_Impl_  { s0 : form   } { s1 : form   } { t0 : form   } { t1 : form   } (H1 : s0 = t0) (H2 : s1 = t1) : Impl_  s0 s1 = Impl_  t0 t1 .
 Proof. congruence. Qed.
 
-Variable retract_ren_form : forall   (xiterm : ( fin ) -> fin) s, ren_form xiterm (inj s) = ren_form_imp xiterm s.
+(* Variable retract_ren_form : forall   (xiterm : ( fin ) -> fin) s, ren_form xiterm (inj s) = ren_form_implicative xiterm s. *)
 
-Definition subst_form_imp   (sigmaterm : ( fin ) -> term ) (s : form_imp ) : form  :=
+Definition subst_form_implicative   (sigmaterm : ( fin ) -> term ) (s : form_implicative ) : form  :=
     match s return form  with
     | Fal   => Fal_ 
     | Impl  s0 s1 => Impl_  ((subst_form sigmaterm) s0) ((subst_form sigmaterm) s1)
     end.
 
-Variable retract_subst_form : forall   (sigmaterm : ( fin ) -> term ) s, subst_form sigmaterm (inj s) = subst_form_imp sigmaterm s.
+Variable retract_subst_form : forall   (sigmaterm : ( fin ) -> term ) s, subst_form sigmaterm (inj s) = subst_form_implicative sigmaterm s.
 
-Definition idSubst_form_imp  (sigmaterm : ( fin ) -> term ) (Eqterm : forall x, sigmaterm x = (var_term ) x) (s : form_imp ) : subst_form_imp sigmaterm s = inj s :=
-    match s return subst_form_imp sigmaterm s = inj s with
+Definition idSubst_form_implicative  (sigmaterm : ( fin ) -> term ) (Eqterm : forall x, sigmaterm x = (var_term ) x) (s : form_implicative ) : subst_form_implicative sigmaterm s = inj s :=
+    match s return subst_form_implicative sigmaterm s = inj s with
     | Fal   => congr_Fal_ 
     | Impl  s0 s1 => congr_Impl_ ((idSubst_form sigmaterm Eqterm) s0) ((idSubst_form sigmaterm Eqterm) s1)
     end.
 
-Definition ext_form_imp   (sigmaterm : ( fin ) -> term ) (tauterm : ( fin ) -> term ) (Eqterm : forall x, sigmaterm x = tauterm x) (s : form_imp ) : subst_form_imp sigmaterm s = subst_form_imp tauterm s :=
-    match s return subst_form_imp sigmaterm s = subst_form_imp tauterm s with
+Definition ext_form_implicative   (sigmaterm : ( fin ) -> term ) (tauterm : ( fin ) -> term ) (Eqterm : forall x, sigmaterm x = tauterm x) (s : form_implicative ) : subst_form_implicative sigmaterm s = subst_form_implicative tauterm s :=
+    match s return subst_form_implicative sigmaterm s = subst_form_implicative tauterm s with
     | Fal   => congr_Fal_ 
     | Impl  s0 s1 => congr_Impl_ ((ext_form sigmaterm tauterm Eqterm) s0) ((ext_form sigmaterm tauterm Eqterm) s1)
     end.
 
-Definition compSubstSubst_form_imp    (sigmaterm : ( fin ) -> term ) (tauterm : ( fin ) -> term ) (thetaterm : ( fin ) -> term ) (Eqterm : forall x, ((funcomp) (subst_term tauterm) sigmaterm) x = thetaterm x) (s : form_imp ) : subst_form tauterm (subst_form_imp sigmaterm s) = subst_form_imp thetaterm s :=
-    match s return subst_form tauterm (subst_form_imp sigmaterm s) = subst_form_imp thetaterm s with
+(* Definition compSubstSubst_form_implicative    (sigmaterm : ( fin ) -> term ) (tauterm : ( fin ) -> term ) (thetaterm : ( fin ) -> term ) (Eqterm : forall x, ((funcomp) (subst_term tauterm) sigmaterm) x = thetaterm x) (s : form_implicative ) : subst_form tauterm (subst_form_implicative sigmaterm s) = subst_form_implicative thetaterm s :=
+    match s return subst_form tauterm (subst_form_implicative sigmaterm s) = subst_form_implicative thetaterm s with
     | Fal   => (eq_trans) (retract_subst_form (_) (Fal )) (congr_Fal_ )
     | Impl  s0 s1 => (eq_trans) (retract_subst_form (_) (Impl (_) (_))) (congr_Impl_ ((compSubstSubst_form sigmaterm tauterm thetaterm Eqterm) s0) ((compSubstSubst_form sigmaterm tauterm thetaterm Eqterm) s1))
     end.
 
-Lemma instId_form_imp  : subst_form_imp (var_term ) = inj .
-Proof. exact ((FunctionalExtensionality.functional_extensionality _ _ ) (fun x => idSubst_form_imp (var_term ) (fun n => eq_refl) ((id) x))). Qed.
+Lemma instId_form_implicative  : subst_form_implicative (var_term ) = inj .
+Proof. exact ((FunctionalExtensionality.functional_extensionality _ _ ) (fun x => idSubst_form_implicative (var_term ) (fun n => eq_refl) ((id) x))). Qed.
 
-Lemma compComp_form_imp    (sigmaterm : ( fin ) -> term ) (tauterm : ( fin ) -> term ) (s : form_imp ) : subst_form tauterm (subst_form_imp sigmaterm s) = subst_form_imp ((funcomp) (subst_term tauterm) sigmaterm) s .
-Proof. exact (compSubstSubst_form_imp sigmaterm tauterm (_) (fun n => eq_refl) s). Qed.
+Lemma compComp_form_implicative    (sigmaterm : ( fin ) -> term ) (tauterm : ( fin ) -> term ) (s : form_implicative ) : subst_form tauterm (subst_form_implicative sigmaterm s) = subst_form_implicative ((funcomp) (subst_term tauterm) sigmaterm) s .
+Proof. exact (compSubstSubst_form_implicative sigmaterm tauterm (_) (fun n => eq_refl) s). Qed.
 
-Lemma compComp'_form_imp    (sigmaterm : ( fin ) -> term ) (tauterm : ( fin ) -> term ) : (funcomp) (subst_form tauterm) (subst_form_imp sigmaterm) = subst_form_imp ((funcomp) (subst_term tauterm) sigmaterm) .
-Proof. exact ((FunctionalExtensionality.functional_extensionality _ _ ) (fun n => compComp_form_imp sigmaterm tauterm n)). Qed.
+Lemma compComp'_form_implicative    (sigmaterm : ( fin ) -> term ) (tauterm : ( fin ) -> term ) : (funcomp) (subst_form tauterm) (subst_form_implicative sigmaterm) = subst_form_implicative ((funcomp) (subst_term tauterm) sigmaterm) .
+Proof. exact ((FunctionalExtensionality.functional_extensionality _ _ ) (fun n => compComp_form_implicative sigmaterm tauterm n)). Qed.
 
-Definition isIn_form_form_imp (s : form) (t : form_imp) : Prop :=
+Definition isIn_form_form_implicative (s : form) (t : form_implicative) : Prop :=
   match t with
-  | Fal  => False
-  | Impl t0 t1 => or (s = t0) (s = t1)
-  end.
- *)
-End form_imp.
+  | Fal   => False
+  | Impl t0 t1  => or (s = t0) (s = t1)
+  end. *)
+
+End form_implicative.
 
 Section form.
 Inductive form  : Type :=
-  | Pred : forall (p : Preds), ( term   ) -> form 
-  | In_form_imp : ( form_imp form  ) -> form 
+  | Pred : forall (p : Preds), ( vect (pred_ar p) (term  ) ) -> form 
+  | In_form_implicative : ( form_implicative form  ) -> form 
   | In_form_univ : ( form_univ form  ) -> form .
-(* 
-Lemma congr_Pred { p : Preds }  { s0 : term   } { t0 : term   } (H1 : s0 = t0) : Pred  p s0 = Pred  p t0 .
+
+Lemma congr_Pred { p : Preds }  { s0 : vect (pred_ar p) (term  ) } { t0 : vect (pred_ar p) (term  ) } (H1 : s0 = t0) : Pred  p s0 = Pred  p t0 .
 Proof. congruence. Qed.
 
-Lemma congr_In_form_imp  { s0 : form_imp form  } { t0 : form_imp form  } (H1 : s0 = t0) : In_form_imp  s0 = In_form_imp  t0 .
+Lemma congr_In_form_implicative  { s0 : form_implicative form  } { t0 : form_implicative form  } (H1 : s0 = t0) : In_form_implicative  s0 = In_form_implicative  t0 .
 Proof. congruence. Qed.
 
 Lemma congr_In_form_univ  { s0 : form_univ form  } { t0 : form_univ form  } (H1 : s0 = t0) : In_form_univ  s0 = In_form_univ  t0 .
 Proof. congruence. Qed.
 
 Global Instance retract_form_univ_form  : retract (form_univ form) form := Build_retract In_form_univ (fun x => match x with
-| In_form_univ s => Datatypes.Some s
+| In_form_univ s  => Datatypes.Some s
 | _ => Datatypes.None
 end) (fun s => eq_refl) (fun s t => match t with
-| In_form_univ t' => fun H => congr_In_form_univ ((eq_sym) (Some_inj H))
+| In_form_univ t'  => fun H => congr_In_form_univ ((eq_sym) (Some_inj H))
 | _ => some_none_explosion
 end) .
 
-Global Instance retract_form_imp_form  : retract (form_imp form) form := Build_retract In_form_imp (fun x => match x with
-| In_form_imp s => Datatypes.Some s
+Global Instance retract_form_implicative_form  : retract (form_implicative form) form := Build_retract In_form_implicative (fun x => match x with
+| In_form_implicative s  => Datatypes.Some s
 | _ => Datatypes.None
 end) (fun s => eq_refl) (fun s t => match t with
-| In_form_imp t' => fun H => congr_In_form_imp ((eq_sym) (Some_inj H))
+| In_form_implicative t'  => fun H => congr_In_form_implicative ((eq_sym) (Some_inj H))
 | _ => some_none_explosion
 end) .
 
-Fixpoint subst_form   (sigmaterm : ( fin ) -> term ) (s : form ) : form  :=
+(* Fixpoint subst_form   (sigmaterm : ( fin ) -> term ) (s : form ) : form  :=
     match s return form  with
-    | Pred  p s0 =>   p ((subst_term sigmaterm) s0)
-    | In_form_imp  s0 =>   ((subst_form_imp (_) subst_form (_) sigmaterm) s0)
-    | In_form_univ  s0 =>   ((subst_form_univ (_) up_term_form subst_form (_) sigmaterm) s0)
+    | Pred  p s0 =>   p ((vect_map (subst_term sigmaterm)) s0)
+    | In_form_implicative  s0 =>   ((subst_form_implicative form sigmaterm) s0)
+    | In_form_univ  s0 =>   ((subst_form_univ form up_term_form sigmaterm) s0)
     end.
 
 Fixpoint idSubst_form  (sigmaterm : ( fin ) -> term ) (Eqterm : forall x, sigmaterm x = (var_term ) x) (s : form ) : subst_form sigmaterm s = s :=
     match s return subst_form sigmaterm s = s with
-    | Pred  p s0 =>  ((idSubst_term sigmaterm Eqterm) s0)
-    | In_form_imp  s0 =>  ((idSubst_form_imp (_) subst_form idSubst_form (_) sigmaterm Eqterm) s0)
-    | In_form_univ  s0 =>  ((idSubst_form_univ (_) up_term_form subst_form upId_term_form idSubst_form (_) sigmaterm Eqterm) s0)
+    | Pred  p s0 =>  ((vect_id (idSubst_term sigmaterm Eqterm)) s0)
+    | In_form_implicative  s0 =>  ((idSubst_form_implicative form sigmaterm Eqterm) s0)
+    | In_form_univ  s0 =>  ((idSubst_form_univ form up_term_form upId_term_form sigmaterm Eqterm) s0)
     end.
 
 Fixpoint ext_form   (sigmaterm : ( fin ) -> term ) (tauterm : ( fin ) -> term ) (Eqterm : forall x, sigmaterm x = tauterm x) (s : form ) : subst_form sigmaterm s = subst_form tauterm s :=
     match s return subst_form sigmaterm s = subst_form tauterm s with
-    | Pred  p s0 =>  ((ext_term sigmaterm tauterm Eqterm) s0)
-    | In_form_imp  s0 =>  ((ext_form_imp (_) subst_form ext_form (_) sigmaterm tauterm Eqterm) s0)
-    | In_form_univ  s0 =>  ((ext_form_univ (_) up_term_form subst_form upExt_term_form ext_form (_) sigmaterm tauterm Eqterm) s0)
+    | Pred  p s0 =>  ((vect_ext (ext_term sigmaterm tauterm Eqterm)) s0)
+    | In_form_implicative  s0 =>  ((ext_form_implicative form sigmaterm tauterm Eqterm) s0)
+    | In_form_univ  s0 =>  ((ext_form_univ form up_term_form upExt_term_form sigmaterm tauterm Eqterm) s0)
     end.
 
 Fixpoint compSubstSubst_form    (sigmaterm : ( fin ) -> term ) (tauterm : ( fin ) -> term ) (thetaterm : ( fin ) -> term ) (Eqterm : forall x, ((funcomp) (subst_term tauterm) sigmaterm) x = thetaterm x) (s : form ) : subst_form tauterm (subst_form sigmaterm s) = subst_form thetaterm s :=
     match s return subst_form tauterm (subst_form sigmaterm s) = subst_form thetaterm s with
-    | Pred  p s0 =>  ((compSubstSubst_term sigmaterm tauterm thetaterm Eqterm) s0)
-    | In_form_imp  s0 =>  ((compSubstSubst_form_imp (_) (_) compSubstSubst_form (_) (fun x y => eq_refl) sigmaterm tauterm thetaterm Eqterm) s0)
-    | In_form_univ  s0 =>  ((compSubstSubst_form_univ (_) up_term_form (_) up_subst_subst_term_form compSubstSubst_form (_) (fun x y => eq_refl) sigmaterm tauterm thetaterm Eqterm) s0)
+    | Pred  p s0 =>  ((vect_comp (compSubstSubst_term sigmaterm tauterm thetaterm Eqterm)) s0)
+    | In_form_implicative  s0 =>  ((compSubstSubst_form_implicative form sigmaterm tauterm thetaterm Eqterm) s0)
+    | In_form_univ  s0 =>  ((compSubstSubst_form_univ form up_term_form up_subst_subst_term_form sigmaterm tauterm thetaterm Eqterm) s0)
     end.
 
 Lemma instId_form  : subst_form (var_term ) = id .
@@ -275,8 +274,8 @@ Lemma compComp_form    (sigmaterm : ( fin ) -> term ) (tauterm : ( fin ) -> term
 Proof. exact (compSubstSubst_form sigmaterm tauterm (_) (fun n => eq_refl) s). Qed.
 
 Lemma compComp'_form    (sigmaterm : ( fin ) -> term ) (tauterm : ( fin ) -> term ) : (funcomp) (subst_form tauterm) (subst_form sigmaterm) = subst_form ((funcomp) (subst_term tauterm) sigmaterm) .
-Proof. exact ((FunctionalExtensionality.functional_extensionality _ _ ) (fun n => compComp_form sigmaterm tauterm n)). Qed.
- *)
+Proof. exact ((FunctionalExtensionality.functional_extensionality _ _ ) (fun n => compComp_form sigmaterm tauterm n)). Qed. *)
+
 End form.
 
 
@@ -294,10 +293,12 @@ End form.
 
 
 
-(***
+
+
+
 Global Instance Subst_term   : Subst1 (( fin ) -> term ) (term ) (term ) := @subst_term   .
 
-Global Instance Subst_form   : Subst1 (( fin ) -> term ) (form ) (form ) := @subst_form   .
+(* Global Instance Subst_form   : Subst1 (( fin ) -> term ) (form ) (form ) := @subst_form   . *)
 
 Global Instance VarInstance_term  : Var (fin) (term ) := @var_term  .
 
@@ -323,11 +324,11 @@ Notation "s [ sigmaterm ]" := (subst_form_univ sigmaterm s) (at level 7, left as
 
 Notation "[ sigmaterm ]" := (subst_form_univ sigmaterm) (at level 1, left associativity, only printing) : fscope.
 
-Notation "s [ sigmaterm ]" := (subst_form_imp sigmaterm s) (at level 7, left associativity, only printing) : subst_scope.
+Notation "s [ sigmaterm ]" := (subst_form_implicative sigmaterm s) (at level 7, left associativity, only printing) : subst_scope.
 
-Notation "[ sigmaterm ]" := (subst_form_imp sigmaterm) (at level 1, left associativity, only printing) : fscope.
+Notation "[ sigmaterm ]" := (subst_form_implicative sigmaterm) (at level 1, left associativity, only printing) : fscope.
 
-Notation "s [ sigmaterm ]" := (subst_form sigmaterm s) (at level 7, left associativity, only printing) : subst_scope.
+(* Notation "s [ sigmaterm ]" := (subst_form sigmaterm s) (at level 7, left associativity, only printing) : subst_scope.
 
 Notation "[ sigmaterm ]" := (subst_form sigmaterm) (at level 1, left associativity, only printing) : fscope.
 
@@ -335,7 +336,7 @@ Ltac auto_unfold := repeat unfold subst1,  subst2,  Subst1,  Subst2,  ids,  ren1
 
 Tactic Notation "auto_unfold" "in" "*" := repeat unfold subst1,  subst2,  Subst1,  Subst2,  ids,  ren1,  ren2,  Ren1,  Ren2,  Subst_term,  Subst_form,  VarInstance_term in *.
 
-Ltac asimpl' := repeat first [progress rewrite ?instId_term| progress rewrite ?compComp_term| progress rewrite ?compComp'_term| progress rewrite ?instId_form_univ| progress rewrite ?compComp_form_univ| progress rewrite ?compComp'_form_univ| progress rewrite ?instId_form_imp| progress rewrite ?compComp_form_imp| progress rewrite ?compComp'_form_imp| progress rewrite ?instId_form| progress rewrite ?compComp_form| progress rewrite ?compComp'_form| progress rewrite ?varL_term| progress (unfold up_ren, up_term_term)| progress (cbn [subst_term subst_form_univ subst_form_imp subst_form])| fsimpl].
+Ltac asimpl' := repeat first [progress rewrite ?instId_term| progress rewrite ?compComp_term| progress rewrite ?compComp'_term| progress rewrite ?instId_form_univ| progress rewrite ?compComp_form_univ| progress rewrite ?compComp'_form_univ| progress rewrite ?instId_form_implicative| progress rewrite ?compComp_form_implicative| progress rewrite ?compComp'_form_implicative| progress rewrite ?instId_form| progress rewrite ?compComp_form| progress rewrite ?compComp'_form| progress rewrite ?varL_term| progress (unfold up_ren, up_term_term)| progress (cbn [subst_term subst_form_univ subst_form_implicative subst_form])| fsimpl].
 
 Ltac asimpl := repeat try unfold_funcomp; auto_unfold in *; asimpl'; repeat try unfold_funcomp.
 
@@ -343,9 +344,8 @@ Tactic Notation "asimpl" "in" hyp(J) := revert J; asimpl; intros J.
 
 Tactic Notation "auto_case" := auto_case (asimpl; cbn; eauto).
 
-Tactic Notation "asimpl" "in" "*" := auto_unfold in *; repeat first [progress rewrite ?instId_term in *| progress rewrite ?compComp_term in *| progress rewrite ?compComp'_term in *| progress rewrite ?instId_form_univ in *| progress rewrite ?compComp_form_univ in *| progress rewrite ?compComp'_form_univ in *| progress rewrite ?instId_form_imp in *| progress rewrite ?compComp_form_imp in *| progress rewrite ?compComp'_form_imp in *| progress rewrite ?instId_form in *| progress rewrite ?compComp_form in *| progress rewrite ?compComp'_form in *| progress rewrite ?varL_term in *| progress (unfold up_ren, up_term_term in * )| progress (cbn [subst_term subst_form_univ subst_form_imp subst_form] in * )| fsimpl in *].
+Tactic Notation "asimpl" "in" "*" := auto_unfold in *; repeat first [progress rewrite ?instId_term in *| progress rewrite ?compComp_term in *| progress rewrite ?compComp'_term in *| progress rewrite ?instId_form_univ in *| progress rewrite ?compComp_form_univ in *| progress rewrite ?compComp'_form_univ in *| progress rewrite ?instId_form_implicative in *| progress rewrite ?compComp_form_implicative in *| progress rewrite ?compComp'_form_implicative in *| progress rewrite ?instId_form in *| progress rewrite ?compComp_form in *| progress rewrite ?compComp'_form in *| progress rewrite ?varL_term in *| progress (unfold up_ren, up_term_term in * )| progress (cbn [subst_term subst_form_univ subst_form_implicative subst_form] in * )| fsimpl in *].
 
 Ltac substify := auto_unfold.
 
-Ltac renamify := auto_unfold.
-*)
+Ltac renamify := auto_unfold. *)
