FOL.v
@@ -2,18 +2,30 @@ Require Export syntax.
 
 Section implicative.
 
-  Notation "« p »" := (In_form_imp p).
-  Notation "p ~> q" := (Impl _ «p» «q») (at level 60).
+  Variable form : Type.
+  
+  Variable count : form -> nat.
+
+  Variable nd : list form -> form -> Prop.
+  Notation "A ⊢ p" := (nd A p) (at level 70).
+  Variable ndHyp : forall A p, In p A -> A ⊢ p.
+
+(*   Notation "« p »" := (In_form_implicative p).
+  Notation "p ~> q" := (Impl _ «p» «q») (at level 60). *)
   Notation "⊥" := (Fal _).
   Notation "¬ p" := (p ~> ⊥) (at level 60).
 
+  Definition count_imp (p : form_implicative form) := match p with
+    | ⊥ => 1
+    | Impl _ p q => count p + count q
+  end.
+
   Reserved Notation "A |- p" (at level 70).
-  Inductive nd (A : list (form_imp form)) : form_imp form -> Prop :=
-    | ndHyp p : In p A -> A |- p
-    | ndExp p : A |- ⊥  -> A |- p
-    | ndII p q : p :: A |- q -> A |- p ~> q
-    | ndIE p q : A |- p ~> q -> A |- p  -> A |- q
-  where "A |- p" := (nd A p).
+  Inductive nd_imp (A : list (form_implicative form)) : form_implicative form -> Prop :=
+    | ndExp p : A |- ⊥ -> A |- p
+    | ndII p q : (p :: A) |- q -> A |- p ~> q
+    | ndIE p q : A |- p ~> q -> A |- p -> A |- q
+  where "A |- p" := (nd_imp A p).
 
   Lemma weakening A B p : A |- p -> incl A B -> B |- p.
   Proof. induction 1; intro Hinc.
@@ -39,8 +51,20 @@ End implicative.
 
 Section universals.
 
+  Variable form : Type.
+    
+  Variable count : form -> nat.
+  Notation "| p |" := count p.
+
+  Variable nd : list form -> form -> Prop.
+  Notation "A ⊢ p" := (nd A p).
+
   Notation "« p »" := (In_form_univ p).
-  Notation "∀ p ":= (All _ «p») (at level 60).
+  Notation "∀ p ":= (All _ p) (at level 60).
+
+  Definition count_univ (p : form_univ form) : nat := match p with 
+    | ∀ p => |p|
+  end.
 
   Definition shifted : list (form_univ form) -> list (form_univ form)
     := fun l => l.
